Veritas.Verifier.Correctness.fst
@@ -17,18 +17,18 @@ open Veritas.Verifier
 type tid (p:pos) = id:nat{id < p}
 
 (* does the log leave the verifier thread in a valid state *)
-let t_verifiable (#p:pos) (#id: tid p)  (l: vlog #p) = Valid? (verifier_thread l id)
+let t_verifiable (#p:pos) (id: tid p)  (l: vlog #p) = Valid? (t_verify id l)
 
 (* refinement types of valid thread-level logs *)
-type t_verifiable_log (#p:pos) (#id: tid p) = l:(vlog #p){t_verifiable #p #id l}
+type t_verifiable_log (#p:pos) (id: tid p) = l:(vlog #p){t_verifiable id l}
 
 (* Full collection of verifier logs one per thread *)
 type g_vlog (#p:pos) = ss:seq (vlog #p){length ss <= p}
 
 (* globally verifiable logs *)
 type g_verifiable (#p:pos) (lg:g_vlog #p) = 
-  forall (i:nat{i < length lg}). {:pattern t_verifiable #p #i (index lg i)} 
-  t_verifiable #p #i (index lg i)
+  forall (i:nat{i < length lg}). {:pattern t_verifiable #p i (index lg i)} 
+  t_verifiable i (index lg i)
 
 (* Refinement type of logs that are verifiable *)
 type g_verifiable_log (#p:pos) = l:g_vlog{g_verifiable #p l}
@@ -43,8 +43,8 @@ let rec g_hadd (#p:pos) (lg:g_verifiable_log #p) (e:nat)
     let hv' = g_hadd lg' e in
     let l = index lg (n - 1) in
     // TODO: how to remove this side-effect assert?
-    assert(t_verifiable #p #(n - 1) l);
-    let h = thread_hadd (verifier_thread l (n - 1)) e in
+    assert(t_verifiable (n - 1) l);
+    let h = thread_hadd (t_verify (n-1) l) e in
     ms_hashfn_agg hv' h  
 
 (* aggregate hadd over all verifier threads *)
@@ -57,8 +57,8 @@ let rec g_hevict (#p:pos) (lg:g_verifiable_log #p) (e:nat)
     let hv' = g_hevict lg' e in
     let l = index lg (n - 1) in
     // TODO: how to remove this side-effect assert?
-    assert(t_verifiable #p #(n - 1) l);
-    let h = thread_hevict (verifier_thread l (n - 1)) e in
+    assert(t_verifiable  (n - 1) l);
+    let h = thread_hevict (t_verify (n- 1) l) e in
     ms_hashfn_agg hv' h  
 
 (* verifiable logs where the first e epochs have identical hadd and hevict *)
@@ -66,31 +66,31 @@ let ep_verifieable_log (#p:pos) (ep:pos) =
   l:(g_verifiable_log #p){forall (e:nat{e < ep}). g_hadd l e = g_hevict l e}
 
 (* the clock of a verifier thread after processing a verfiable log *)
-let clock_after (#p:pos) (#id:tid p) (l:t_verifiable_log #p #id) = 
-  let vs = verifier_thread l id in
+let clock_after (#p:pos) (#id:tid p) (l:t_verifiable_log id) = 
+  let vs = t_verify id l in
   Valid?.clk vs
 
 let rec lemma_verifiable_implies_prefix_verifiable
-  (#p:pos) (#id:tid p) (l:t_verifiable_log #p #id) (i:nat{i <= length l}):
+  (#p:pos) (id:tid p) (l:t_verifiable_log id) (i:nat{i <= length l}):
   Lemma (requires (True))
-        (ensures (t_verifiable #p #id (prefix l i)))
+        (ensures (t_verifiable id (prefix l i)))
         (decreases (length l)) 
         =
   let n = length l in
   if n = 0 then ()
   else if i = n then ()
   else
-    lemma_verifiable_implies_prefix_verifiable #p #id (prefix l (n - 1)) i
+    lemma_verifiable_implies_prefix_verifiable id (prefix l (n - 1)) i
 
 (* TODO: Adding SMTPat (prefix l i) does not work in the lemma_above *)
-let t_vprefix (#p:pos) (#id:tid p) (l:t_verifiable_log #p #id) (i:nat{i <= length l}): 
-  l':(t_verifiable_log #p #id){l' = prefix l i} = 
+let t_vprefix (#p:pos) (#id:tid p) (l:t_verifiable_log id) (i:nat{i <= length l}): 
+  l':(t_verifiable_log id){l' = prefix l i} = 
   let l' = prefix l i in
-  lemma_verifiable_implies_prefix_verifiable l i;
+  lemma_verifiable_implies_prefix_verifiable id l i;
   l'
 
 (* the clock of a verifier is monotonic *)
-let rec lemma_clock_monotonic (#p:pos) (#id:tid p) (l:t_verifiable_log #p #id)
+let rec lemma_clock_monotonic (#p:pos) (#id:tid p) (l:t_verifiable_log id)
                           (i:nat{i <= length l}):
   Lemma (requires(True))
         (ensures (clock_after (t_vprefix l i) `ts_leq` clock_after l)) 
@@ -103,6 +103,21 @@ let rec lemma_clock_monotonic (#p:pos) (#id:tid p) (l:t_verifiable_log #p #id)
     let l' = t_vprefix l (n - 1) in
     lemma_clock_monotonic l' i
 
+type clocked_vlog_entry (#p:nat) = vlog_entry #p * timestamp
+
+type clocked_vlog (#p:nat) = seq (clocked_vlog_entry #p)
+
+let rec attach_clock (#p:pos) (id:tid p) (l:t_verifiable_log id): 
+  Tot (clocked_vlog #p) 
+  (decreases (length l)) = 
+  let n = length l in
+  if n = 0 then empty 
+  else 
+    let l' = t_vprefix l (n - 1) in
+    let cl' = attach_clock id l' in
+    let t = clock_after l in
+    let e = index l (n - 1) in
+    append cl' (create 1 (e, t))
 
 (* is s' a prefix of s *)
 let is_prefix (#a:eqtype) (s':seq a) (s:seq a) = 
